implementing concrete bigraphs se

src/ConcreteBigraphs.v
@@ -15,7 +15,7 @@ Require Import FunctionalExtensionality.
 Require Import ProofIrrelevance.
 Require Import PropExtensionality.
 Require Import SignatureBig.
-Require Import Names.
+Require Import InfSets.
 
 
 Require Import Coq.Lists.List.
@@ -36,48 +36,50 @@ Import ListNotations.
 
 (** This module implements bigraphs and basic operations on bigraphs *)
 Module Bigraphs (sp : SignatureParameter) 
-  (np : Names.InfiniteParameter).
+  (np : InfiniteParameter)
+  (vp : InfiniteParameter)
+  (ep : InfiniteParameter).
 Module s := Signature sp.
 Module n := FiniteSubset np.
-Module v := FiniteSubset np.
-Module e := FiniteSubset np.
+Module v := FiniteSubset vp.
+Module e := FiniteSubset ep.
 Include s.
-Include n.
+Import n.
+Import v.
+Import n.
 (** * Definition of a bigraph
   This section defines the Type bigraph *)
 Section IntroBigraphs.
 
-
 Record bigraph  (site: nat) 
-                (innername: NoDupList) 
+                (innername: n.NoDupList) 
                 (root: nat) 
-                (outername: NoDupList) : Type := 
+                (outername: n.NoDupList) : Type := 
   Big  
   { 
-    node : NoDupList ;
-    edge : NoDupList ;
-    control : ListType node -> Kappa ;
-    parent : ListType node + ordinal site -> ListType node + ordinal root ; 
-    link : ListType innername + Port control -> 
-                (ListType outername) + ListType edge; 
+    node : v.NoDupList ;
+    edge : e.NoDupList ;
+    control : v.ListType node -> Kappa ;
+    parent : v.ListType node + ordinal site -> v.ListType node + ordinal root ; 
+    link : n.ListType innername + Port control -> 
+                (ListType outername) + e.ListType edge; 
     ap : FiniteParent parent ;
   }.
-Locate ListType.
 
 End IntroBigraphs.
 
 (** * Getters
   This section is just getters to lightenn some notations *)
 Section GettersBigraphs.
-Definition get_node {s r : nat} {i o : NoDupList} (bg : bigraph s i r o) : NoDupList := 
-  @node s i r o bg.
-Definition get_edge {s r : nat} {i o : NoDupList} (bg : bigraph s i r o) : NoDupList := 
+Definition get_node {s r : nat} {i o : NoDupList} (bg : bigraph s i r o) : v.NoDupList := 
+  (@node s i r o bg).
+Definition get_edge {s r : nat} {i o : NoDupList} (bg : bigraph s i r o) : e.NoDupList := 
   @edge s i r o bg.
-Definition get_control {s r : nat} {i o : NoDupList} (bg : bigraph s i r o) : ListType  -> Kappa :=
+Definition get_control {s r : nat} {i o : NoDupList} (bg : bigraph s i r o) : v.ListType (get_node bg) -> Kappa :=
   @control s i r o bg.
-Definition get_parent {s r : nat} {i o : NoDupList} (bg : bigraph s i r o) : (get_node bg) + (ordinal s) -> (get_node bg) + (ordinal r) :=
+Definition get_parent {s r : nat} {i o : NoDupList} (bg : bigraph s i r o) : v.ListType (get_node bg) + (ordinal s) -> v.ListType (get_node bg) + (ordinal r) :=
   @parent s i r o bg.
-Definition get_link {s r : nat} {i o : NoDupList} (bg : bigraph s i r o) : {inner:InfType | In inner i} + Port (@get_control s r i o bg) -> {outer:InfType | In outer o} + (get_edge bg) :=
+Definition get_link {s r : nat} {i o : NoDupList} (bg : bigraph s i r o) : {inner:InfType | In inner i} + Port (@get_control s r i o bg) -> {outer:InfType | In outer o} + e.ListType (get_edge bg) :=
   @link s i r o bg.
 Definition get_ap {s r : nat} {i o : NoDupList} (bg : bigraph s i r o) : FiniteParent (get_parent (bg:=bg)) := 
   @ap s i r o bg.
@@ -103,13 +105,13 @@ Theorem innername_proof_irrelevant {s i r o} (b:bigraph s i r o):
   intros. apply f_equal. apply f_equal. apply subset_eq_compat. reflexivity.
   Qed.
 Theorem port_proof_irrelevant {s i r o} (b:bigraph s i r o): 
-  forall n n':get_node b, forall port:nat, forall Hport Hport', n=n' ->
+  forall n n':v.ListType (get_node b), forall port:nat, forall Hport Hport', n=n' ->
   get_link (bg:=b) (inr (existT 
-    (fun n : get_node b => 'I_(Arity (get_control (bg:=b) n))) 
+    (fun n : v.ListType (get_node b) => 'I_(Arity (get_control (bg:=b) n))) 
     n
     (Ordinal (n:=Arity (get_control (bg:=b) n)) (m:=port) Hport))) =
   get_link (bg:=b) (inr (existT 
-    (fun n : get_node b => 'I_(Arity (get_control (bg:=b) n))) 
+    (fun n : v.ListType (get_node b) => 'I_(Arity (get_control (bg:=b) n))) 
     n'
     (Ordinal (n:=Arity (get_control (bg:=b) n')) (m:=port) Hport'))).
   Proof. 
@@ -117,7 +119,7 @@ Theorem port_proof_irrelevant {s i r o} (b:bigraph s i r o):
   rewrite (Ordinal_proof_irrelevance _ _ Hport). reflexivity.
   Qed.
 Theorem port_proof_irrelevant_full {s i r o} (b:bigraph s i r o): 
-  forall n n':get_node b, 
+  forall n n':v.ListType (get_node b), 
   forall port : 'I_(Arity (get_control n)),
   forall port': 'I_(Arity (get_control n')), 
   n=n' -> nat_of_ord port = nat_of_ord port' ->
@@ -142,30 +144,31 @@ Theorem port_proof_irrelevant_full {s i r o} (b:bigraph s i r o):
 Section ElementaryBigraphs. 
 Definition bigraph_id (s: nat) (i : NoDupList) : bigraph s i s i. (*actually s i s (permutation i) *)
   Proof.
-  apply (@Big s i s i
-          void (*node : ∅*)
-          void (*edge : ∅*)
-          (@void_univ_embedding _) (*control : ∅_Kappa*)
+  eapply (@Big s i s i
+          v.EmptyNDL (*node : ∅*)
+          e.EmptyNDL (*edge : ∅*)
+          _ (*control : ∅_Kappa*)
           id (*parent : id*)
         ).
+  Unshelve.
   - intros [inner | port]. (*link_|{names} : id*)
     + left. apply inner. 
-    + destruct port. destruct x.
-  - intro n. (*acyclic parent*)
-    destruct n.
+    + destruct port as [[port InPort] Hport]. destruct InPort.
+  - intros [_ []]. (*acyclic parent*)
+  - intros [_ []]. (*control*)
   Defined.
 
 Definition bigraph_empty : bigraph 0 EmptyNDL 0 EmptyNDL := bigraph_id 0 EmptyNDL.
 
 
-Definition discrete_atom {A:finType} 
-  (a:A) {k:Kappa} (o:NoDupList) 
+Definition discrete_atom 
+  (node:vp.InfType) {k:Kappa} (o:NoDupList) 
   {Hkappa : MyEqNat (Arity k) (length (ndlist o))}: bigraph 0 EmptyNDL 1 o.
-  Search (is_true (0 < 1)).
+  Proof.
   eapply (@Big
       0 EmptyNDL 1 o
-      A
-      void
+      (v.OneelNDL node)
+      (e.EmptyNDL)
       (fun n => k) (*control*)
       (fun ns => match ns with 
         | inl n => inr (Ordinal (ltn0Sn 0))
@@ -192,24 +195,30 @@ Definition discrete_atom {A:finType}
     exfalso. discriminate H.
     Defined. 
 
-Definition discrete_ion {A:finType} 
-  (a:A) {k:Kappa} (o:NoDupList) 
+Definition discrete_ion (node:vp.InfType) {k:Kappa} (o:NoDupList) 
   {Hkappa : MyEqNat (Arity k) (length (ndlist o))}: bigraph 1 EmptyNDL 1 o.
+  Proof.
   eapply (@Big
       1 EmptyNDL 1 o
-      A
-      void
+      (v.OneelNDL node)
+      (e.EmptyNDL)
       (fun n => k) (*control*)
       (fun ns => match ns with 
         | inl n => inr (Ordinal (ltn0Sn 0))
-        | inr s => inl a
+        | inr s => _
       end) (*parent*)
       _ (*link*)
     ).
     Unshelve.
-    2:{ intros [i|p].  
-      - destruct i as [i H]. elim H. 
-      - left. unfold ListType. destruct o as [o Ho]. 
+    - unfold FiniteParent. simpl. (*Acyclic Parent*)
+    intros u.
+    apply Acc_intro.
+    intros u' H.
+    exfalso. discriminate H.
+    - left. unfold v.ListType. exists node. constructor. reflexivity. (*parent*)
+    - intros [i|p].  (*link*)
+      + destruct i as [i H]. elim H. 
+      + left. unfold ListType. destruct o as [o Ho]. 
       destruct p as [i H]. destruct H as [p Hp]. 
       exists (Coq.Lists.List.nth p o DefaultInfType). 
       apply nth_In. destruct Hkappa as [Hkappa].
@@ -217,42 +226,40 @@ Definition discrete_ion {A:finType}
       set (tmp := ltP (m:=p) (n:=Arity k)).
       apply Bool.reflect_iff in tmp.      
       rewrite tmp.
-      apply Hp. } (*link*)
-    unfold FiniteParent. simpl.
-    intros u.
-    apply Acc_intro.
-    intros u' H.
-    exfalso. discriminate H.
+      apply Hp. 
     Defined. 
 
 Definition permutationbig (n : nat) : bigraph n EmptyNDL n EmptyNDL. 
   Proof. 
-  apply (@Big n EmptyNDL n EmptyNDL
-    void (*node : ∅*)
-    void (*edge : ∅*)
-    (@void_univ_embedding _) (*control : ∅_-> Kappa*)
-    (fun sn => match sn with |inr s => inr s | inl n => match n with end end) (*parent : sites -> root*)
+  eapply (@Big n EmptyNDL n EmptyNDL
+    v.EmptyNDL (*node : ∅*)
+    e.EmptyNDL (*edge : ∅*)
+    _ (*control : ∅_-> Kappa*)
+    (fun sn => match sn with |inr s => inr s | inl n => _ end) (*parent : sites -> root*)
   ).
-  - intros [inner | port]. (*link : ∅*)
-  + left. apply inner.
-  + destruct port. destruct x.
-  - intro n'. (*acyclic parent*)
-  destruct n'.
+  Unshelve.
+  - intros [[inner Hinner] | [[port Hp] Hport]]. (*link : ∅*)
+    + destruct Hinner.
+    + destruct Hp. 
+  - intros [_ []]. (*acyclic parent*)
+  - intros [_ []]. (*control*)
+  - destruct n as [n []].
   Defined.
 
 Definition merge {n:nat} : bigraph n EmptyNDL 1 EmptyNDL.
   Proof. 
-  apply (@Big n EmptyNDL 1 EmptyNDL
-    void (*node : ∅*)
-    void (*edge : ∅*)
-    (@void_univ_embedding _) (*control : ∅ ->_Kappa*)
+  eapply (@Big n EmptyNDL 1 EmptyNDL
+    v.EmptyNDL (*node : ∅*)
+    e.EmptyNDL (*edge : ∅*)
+    _ (*control : ∅ ->_Kappa*)
     (fun s => inr (Ordinal (ltn0Sn 0))) (*parent : sites -> root*)
   ).
-  - intros [inner | port]. (*link : ∅*)
-  + left. apply inner.
-  + destruct port. destruct x.
-  - intro n'. (*acyclic parent*)
-  destruct n'.
+  Unshelve.
+  - intros [[inner Hinner] | [[port Hp] Hport]]. (*link : ∅*)
+    + destruct Hinner.
+    + destruct Hp. 
+  - intros [_ []]. (*acyclic parent*)
+  - intros [_ []]. (*control*)
   Defined.
 
 Definition big_1 := @merge 0.
@@ -260,60 +267,61 @@ Definition big_1 := @merge 0.
 Definition symmetry_big (m:nat) (X:NoDupList) (n:nat) (Y:NoDupList) :
   bigraph (m+n) (X ∪ Y) (m+n) (X ∪ Y).
   Proof. 
-    eapply (@Big (m+n) (X ∪ Y) (m+n) (X ∪ Y)
-      void (*node : ∅*)
-      void (*edge : ∅*)
-      (@void_univ_embedding _) (*control : ∅ ->_Kappa*)
-      _ _ _
-    ).
-    Unshelve.
-    - intros [v|s]. (*parent*)
-      + destruct v.
-      + right. destruct s as [s Hs].
-      destruct (ltnP s m).
-      * exists (s+n). rewrite ltn_add2r. apply i.
-      * exists (s-m). 
-      set (tmp := leq_subr m s).
-      apply (leq_ltn_trans tmp) in Hs.
-      apply Hs.
-    - intros [inner | port]. (*link : ∅*)
-      + left. apply inner.
-      + destruct port. destruct x.
-    - intro n'. (*acyclic parent*)
-    destruct n'.
+  eapply (@Big (m+n) (X ∪ Y) (m+n) (X ∪ Y)
+  v.EmptyNDL (*node : ∅*)
+  e.EmptyNDL (*edge : ∅*)
+  _ (*control : ∅ ->_Kappa*)
+    _ _ _
+  ).
+  Unshelve.  
+  - intros [_ []]. (*control*)
+  - intros [[_ []]|s]. (*parent*)
+    right. destruct s as [s Hs].
+    destruct (ltnP s m).
+    * exists (s+n). rewrite ltn_add2r. apply i.
+    * exists (s-m). 
+    set (tmp := leq_subr m s).
+    apply (leq_ltn_trans tmp) in Hs.
+    apply Hs.
+  - intros [inner | [[_ []] []]]. (*link : ∅*)
+    left. apply inner.
+  - intros [_ []]. (*acyclic parent*)
   Defined.
 
 Definition substitution (i:NoDupList) (name:InfType) : bigraph 0 i 0 (OneelNDL name).
   Proof. 
-  apply (@Big 0 i 0 (OneelNDL name)
-    void (*node : ∅*)
-    void (*edge : ∅*)
-    (@void_univ_embedding _) (*control : ∅_Kappa*)
-    (void_univ_embedding ||| (void_univ_embedding <o> bij_ord_zero)) (*parent : sites -> root*)
+  eapply (@Big 0 i 0 (OneelNDL name)
+    v.EmptyNDL (*node : ∅*)
+    e.EmptyNDL (*edge : ∅*)
+    _ (*control : ∅_Kappa*)
+    _ (*parent : sites -> root*)
   ).
-  - intros [inner | port]. (*link : ∅*)
-  + left. exists name. simpl. left. reflexivity.
-  + destruct port. destruct x.
-  - intro n'. (*acyclic parent*)
-  destruct n'.
+  Unshelve.
+  - intros [inner | [[_ []] []]]. (*link : ∅*)
+    left. exists name. simpl. left. reflexivity.
+  - intros [_ []]. (*acyclic parent*)
+  - intros [_ []]. (*control*)
+  - intros [[_ []] | [site Hsite]]. (*parent*)
+    discriminate Hsite.
   Defined.
 
 Definition elementary_renaming (n n':InfType) := substitution (OneelNDL n) n'.
 
-
 Definition closure (name:InfType) : bigraph 0 (OneelNDL name) 0 EmptyNDL.
   Proof. 
-  apply (@Big 0 (OneelNDL name) 0 EmptyNDL
-    void (*node : ∅*)
-    unit (*edge : ∅*)
-    (@void_univ_embedding _) (*control : ∅_Kappa*)
-    (void_univ_embedding ||| (void_univ_embedding <o> bij_ord_zero)) (*parent : sites -> root*)
+  eapply (@Big 0 (OneelNDL name) 0 EmptyNDL
+    v.EmptyNDL (*node : ∅*)
+    (e.OneelNDL (e.DefaultInfType)) (*edge : ∅*)
+    _ (*control : ∅_Kappa*)
+    _ (*parent : sites -> root*)
   ).
-  - intros [inner | port]. (*link : ∅*)
-  + right. simpl. exact tt. 
-  + destruct port. destruct x.
-  - intro n'. (*acyclic parent*)
-  destruct n'.
+  Unshelve.
+  - intros [inner | [[_ []] _]]. (*link : ∅*)
+    right. unfold e.ListType. exists e.DefaultInfType. constructor. reflexivity.
+  - intros [_ []]. (*acyclic parent*)
+  - intros [_ []]. (*control*)
+  - intros [[_ []] | [site Hsite]]. (*parent*)
+    discriminate Hsite.
   Defined.
 
 Definition join_big := @merge 2. 
